

MULTIVARIATE NORMAL DISTRIBUTION

$$X: \Omega \rightarrow \mathbb{R}^n \quad X \sim N(\mu, \sigma^2)$$

Let $Z_1, \dots, Z_d \sim N(0, 1)$ INDEPENDENT

Consider the vector $Z = (Z_1, \dots, Z_d)$

$$u \in \mathbb{R}^d, \quad |u| = \sqrt{\sum_{i=1}^d u_i^2} = \sqrt{\langle u, u \rangle}$$

Characteristic function of Z :

$$\begin{aligned} \varphi_Z(u) &= \varphi_Z(u_1, \dots, u_d) = \prod_{i=1}^d \varphi_{Z_i}(u_i) \\ &= \prod_{i=1}^d e^{-\frac{u_i^2}{2}} = e^{-\frac{\sum_{i=1}^d u_i^2}{2}} = e^{-\frac{|u|^2}{2}} \end{aligned}$$

Let $A \in \mathbb{R}^{n \times d}$, $\mu \in \mathbb{R}^n$

$$X = AZ + \mu \quad \text{random vector in } \mathbb{R}^n$$

Compute $\varphi_X(v)$ $v \in \mathbb{R}^n$

$$\begin{aligned} \varphi_X(v) &= e^{i \langle v, \mu \rangle} \cdot \varphi_Z(A^T v) \\ &= e^{i \langle v, \mu \rangle} e^{-\frac{|A^T v|^2}{2}} \end{aligned}$$

$$\begin{aligned} |A^T v|^2 &= \langle A^T v, A^T v \rangle = (A^T v)^T A^T v \\ &= v^T \underbrace{(A^T)^T}_A A^T v = v^T (A A^T v) = \langle v, A A^T v \rangle \end{aligned}$$

Denote $\Sigma = A A^T$ $\Sigma \in \mathbb{R}^{n \times n}$

Properties

- Σ is symmetric.

$$\Sigma^T = (A A^T)^T = (A^T)^T A^T = A A^T = \Sigma$$

- Σ is POSITIVE SEMIDEFINITE,

$$\text{i.e. } \langle v, \Sigma v \rangle \geq 0 \quad \forall v \in \mathbb{R}^n$$

$$\text{in fact } \langle v, \Sigma v \rangle = |A^T v|^2 \geq 0$$

$$\varphi_X(v) = e^{-i \langle v, \mu \rangle} e^{-\frac{1}{2} |v|^2}$$

- Expectation of X :

$$A = (a_{ij})_{\substack{i=1, \dots, n \\ j=1, \dots, d}}$$

$$\begin{pmatrix} | & X_1 & | \end{pmatrix} \quad \begin{pmatrix} | & \in & | & X_1 & | \end{pmatrix}$$

- Expectation of X : $A = (a_{ij})_{i=1, \dots, n}^{j=1, \dots, d}$

$$E[X] = E[AZ + \mu] = E\left[\begin{pmatrix} X_1 \\ \vdots \\ X_d \end{pmatrix}\right] = \begin{pmatrix} E[X_1] \\ \vdots \\ E[X_d] \end{pmatrix}$$

$$E[X_i] = E\left[\sum_{j=1}^d a_{ij} Z_j + \mu_i\right]$$

$$= \sum_{j=1}^d a_{ij} \underbrace{E[Z_j]}_{=0} + E[\mu_i] = \mu_i$$

$$\Rightarrow E[X] = \mu$$

- Compute Covariances

$$\text{Cov}(X_i, X_j) = E[(X_i - \underbrace{E[X_i]}_{=\mu_i})(X_j - \underbrace{E[X_j]}_{=\mu_j})]$$

$$= E\left[\sum_{k=1}^d a_{ik} Z_k \cdot \sum_{l=1}^d a_{jl} Z_l\right]$$

$$= \sum_{k=1}^d a_{ik} \sum_{l=1}^d a_{jl} E[Z_k Z_l]$$

$$E[Z_k Z_l] = \begin{cases} E[Z_k^2] = 1 & \text{if } k=l \\ E[Z_k] \cdot E[Z_l] = 0 & \text{if } k \neq l \end{cases}$$

$$= \sum_{k=1}^d a_{ik} a_{jk} = (A A^T)_{ij} = \Sigma_{ij}$$

$$\Rightarrow \text{Cov}(X_i, X_j) = \Sigma_{ij}$$

$$\Sigma \text{ is called the COVARIANCE MATRIX}$$

Def A random vector X is called NORMAL with mean μ and covariance matrix Σ (Σ symmetric and positive semidefinite) if its characteristic function is equal to

$$\varphi_X(v) = e^{i \langle v, \mu \rangle} e^{-\frac{1}{2} \langle \Sigma v, v \rangle}$$

and we denote $X \sim N(\mu, \Sigma)$

- Z standard if $Z \sim N(0, Id)$

Proposition 1

Proposition 1

Let $X \sim N(\mu, \Sigma)$ and let $Y = BX + b$
then $Y \sim N(B\mu + b, B\Sigma B^T)$

Proposition 2

If (X, Y) is a 2-dimensional normal vector. Then
 $X \perp Y \iff \text{Cov}(X, Y) = 0$

Proof

(\Rightarrow) always true

(\Leftarrow) We have to show that

X and Y uncorrelated $\Rightarrow X \perp Y$

$$\text{Covariance matrix } \Sigma = \begin{pmatrix} \text{Cov}(X, X) & \text{Cov}(X, Y) \\ \text{Cov}(X, Y) & \text{Cov}(Y, Y) \end{pmatrix}$$
$$\Sigma = \begin{pmatrix} \sigma_x^2 & 0 \\ 0 & \sigma_y^2 \end{pmatrix} \quad \begin{matrix} \mu_x = E[X], & \mu_y = E[Y] \\ \sigma_x^2 = \text{Var}(X), & \sigma_y^2 = \text{Var}(Y) \end{matrix}$$

$$\begin{aligned} \varphi_{X,Y}(u, v) &= \exp(i \langle (u, v), (\mu_x, \mu_y) \rangle) \exp\left(-\frac{1}{2} \langle \Sigma \begin{pmatrix} u \\ v \end{pmatrix}, \begin{pmatrix} u \\ v \end{pmatrix} \rangle\right) \\ &= \exp(i(u\mu_x + v\mu_y)) \exp\left(-\frac{1}{2}(\sigma_x^2 u^2 + \sigma_y^2 v^2)\right) \\ \left| \langle \Sigma \begin{pmatrix} u \\ v \end{pmatrix}, \begin{pmatrix} u \\ v \end{pmatrix} \rangle = \left\langle \begin{pmatrix} \sigma_x^2 & 0 \\ 0 & \sigma_y^2 \end{pmatrix} \begin{pmatrix} u \\ v \end{pmatrix}, \begin{pmatrix} u \\ v \end{pmatrix} \right\rangle = \left\langle \begin{pmatrix} \sigma_x^2 u \\ \sigma_y^2 v \end{pmatrix}, \begin{pmatrix} u \\ v \end{pmatrix} \right\rangle \right. \\ &= e^{i u \mu_x} e^{i v \mu_y} e^{-\frac{1}{2} \sigma_x^2 u^2} e^{-\frac{1}{2} \sigma_y^2 v^2} \\ &= e^{i u \mu_x - \frac{1}{2} \sigma_x^2 u^2} e^{i v \mu_y - \frac{1}{2} \sigma_y^2 v^2} \\ &= \varphi_X(u) \varphi_Y(v) \end{aligned}$$

Then $X \perp Y$, as $\varphi_{X,Y}(u, v) = \varphi_X(u) \varphi_Y(v)$ \square

Remark

- In scalar case $\mu \in \mathbb{R}$, $\Sigma = \sigma^2 \in \mathbb{R}$
 $N(\mu, \sigma^2)$ is usual normal distribution on \mathbb{R}
- Σ is covariance matrix in the sense that
 $\Sigma_{ij} = \text{Cov}(X_i, X_j)$ if $X \sim N(\mu, \Sigma)$

$$\Sigma_{ij} = \text{Cov}(X_i, X_j) \quad \text{if } X \sim N(\mu, \Sigma)$$

Note The vector $X \sim N(\mu, \Sigma)$ might not be absolutely continuous

Result $X \sim N(\mu, \Sigma)$ multivariate normal random vector in \mathbb{R}^n
 X is absolutely continuous $\Leftrightarrow \det(\Sigma) \neq 0$

In this case the density of X is (Σ is invertible)

$$f_X(x) = \frac{1}{(2\pi)^{\frac{n}{2}} |\det \Sigma|} \exp\left(-\frac{1}{2} \langle x, \Sigma^{-1} x \rangle\right)$$

A such that $X = AZ + \mu$

Exercise

$$X_1 \sim U(0,1)$$

$$F_{X_1}(x) = x \quad \text{if } 0 \leq x \leq 1$$

$$Z = \max(X_1, \dots, X_n) \quad X_1, \dots, X_n \text{ INDEPENDENT}$$

$$F_Z(z) = \prod_{i=1}^n F_{X_i}(z) = \prod_{i=1}^n z = z^n \quad 0 \leq z \leq 1$$

$$F_Z(z) = \begin{cases} 0 & z \leq 0 \\ 1 & z \geq 1 \end{cases}$$

$$E[Z] = \int_0^{+\infty} (1 - F_Z(z)) dz$$

$$\text{or } F_Z' = f_Z \quad E[Z] = \int_0^{+\infty} z f_Z(z) dz$$

$$\begin{aligned} E[Z] &= \int_0^1 (1 - F_Z(z)) dz + \int_1^{+\infty} (1 - F_Z(z)) dz \\ &= \int_0^1 (1 - z^n) dz + 0 \\ &= 1 - \left[\frac{z^{n+1}}{n+1} \right]_0^1 = 1 - \frac{1}{n+1} = \frac{n}{n+1} \end{aligned}$$

• Alternatively

$$\begin{aligned} f_Z(z) &= F_Z'(z) = n z^{n-1} \mathbb{1}_{[0,1]}^{(z)} \\ E[Z] &= \int_0^{+\infty} z f_Z(z) dz = \int_0^1 z n z^{n-1} dz = n \int_0^1 z^n dz \\ &= n \left[\frac{z^{n+1}}{n+1} \right]_0^1 = \frac{n}{n+1} \end{aligned}$$

$$= \frac{1}{n} \left[\frac{z^{n+1}}{n+1} \right]_0^1 = \frac{n}{n+1}$$

$$W = \max(X_1, \dots, X_n)$$

$$\begin{aligned} F_W(w) &= 1 - \prod_{i=1}^n (1 - F_{X_i}(w)) \\ &= 1 - (1 - w)^n \quad \text{if } 0 \leq w \leq 1 \\ &= \begin{cases} 0 & \text{if } w \leq 0 \\ 1 & \text{if } w \geq 1 \end{cases} \end{aligned}$$

$$\begin{aligned} E[W] &= \int_0^{\infty} (1 - F_W(w)) dw \\ &= \int_0^1 (1 - w)^n dw = \left[-\frac{(1 - w)^{n+1}}{n+1} \right]_{w=0}^{w=1} \\ &= \frac{1}{n+1} \end{aligned}$$